# Solution-3

1. 

   a) $T\implies D\and Y$ 

   b) $D\implies\neg Y$

   c) $\neg D\implies \neg T$

   d) $T\implies \neg (D \and  Y)$

   e) $\neg D \and  Y \and T$ 

   f) $T \implies (Y \implies \neg D)$

   g) $T \implies (D \implies  Y) \or (Y \implies  D)$

   h) $T \implies (D \or  Y) \and \neg (D \or Y)$ 

2. 

   | $\phi$ | $\neg \phi $ | $\psi$ | $\phi\implies\psi$ | $\neg\phi\or\psi$ |
   | ------ | ------------ | ------ | ------------------ | ----------------- |
   | T      | F            | T      | T                  | T                 |
   | T      | F            | F      | F                  | F                 |
   | F      | T            | T      | T                  | T                 |
   | F      | T            | F      | T                  | T                 |

3. The truth value of $\phi\implies\psi$ is equivalent to  $\neg\phi\or\psi$.

4. | $ \phi $ | $ \psi $ | $ \neg \psi $ | $\phi \implies \psi $ | $\phi \nRightarrow \psi $ | $\phi \and \neg \psi$ |
   | -------- | -------- | ------------- | --------------------- | ------------------------- | --------------------- |
   | T        | T        | F             | T                     | F                         | F                     |
   | T        | F        | T             | F                     | T                         | T                     |
   | F        | T        | F             | T                     | F                         | F                     |
   | F        | F        | T             | T                     | F                         | F                     |

5. The truth value of $\phi \nRightarrow \psi $ is equivalent to $\phi \and \neg \psi$.